update

Test/civl/duplicate.bpl
@@ -28,29 +28,29 @@ function {:inline} {:linear "addr2"} IntsCollector2(xs: [int]bool) : [int]bool
   xs
 }
 
-var {:layer 0,3} {:linear} Addrs:[int]bool;  // ghost
-var {:layer 0,3} done: [int]bool;
+var {:layer 0,3} {:linear "addr1"} Addrs:[int]bool;  // ghost
+var {:layer 0,3} done: [int]int;
 var {:layer 0,4} x:[int]int;
 
-procedure {:yields} {:layer 0} {:refines "AtomicDoneUpdate"} DoneUpdate(i: int) returns ({:linear "addr1"} x: Addr);
-procedure {:atomic} {:layer 1} AtomicDoneUpdate(i: int) returns ({:linear "addr1"} x: Addr)
+procedure {:yields} {:layer 0} {:refines "AtomicDoneUpdate"} DoneUpdate(i: int, phase: int) returns ({:linear "addr1"} x: Addr);
+procedure {:atomic} {:layer 1} AtomicDoneUpdate(i: int, phase: int) returns ({:linear "addr1"} x: Addr)
 modifies done, Addrs;
 {
-    if (done[i]) {
+    if (done[i] >= phase) {
         x := None();
     } else {
-        done[i] := true;
+        done[i] := phase;
 	Addrs[i] := false;
 	x := Some(i);
     }
 }
 
-procedure {:yields} {:layer 0} {:refines "AtomicAddAddr"} AddAddr({:linear_in "addr1"} i1: int, {:linear "addr2"} i2: int);
-procedure {:atomic} {:layer 3} AtomicAddAddr({:linear_in "addr1"} i1: int, {:linear "addr2"} i2: int)
+procedure {:yields} {:layer 0} {:refines "AtomicAddAddr"} AddAddr({:linear_in "addr1"} i1: int, {:linear "addr2"} i2: int, phase: int);
+procedure {:atomic} {:layer 1,3} AtomicAddAddr({:linear_in "addr1"} i1: int, {:linear "addr2"} i2: int, phase: int)
 modifies Addrs;
 {
     assert i1 == i2;
-    assert !done[i1];
+    assert done[i1] < phase;
     Addrs[i1] := true;
 }
 
@@ -75,12 +75,12 @@ modifies x;
     x[i] := 2*x[i];
 }
 
-procedure {:yields} {:layer 1} {:refines "AtomicRemoteIncrementBody"} RemoteIncrementBody(i: int)
+procedure {:yields} {:layer 1} {:refines "AtomicRemoteIncrementBody"} RemoteIncrementBody(i: int, phase: int)
 {
     var {:linear "addr1"} j: int;
     var {:linear "addr1"} x: Addr;
     yield;
-    call x := DoneUpdate(i);
+    call x := DoneUpdate(i, phase);
     if (is#Some(x)) {
         call j := Extract(x);   
         call Increment(j);
@@ -88,35 +88,35 @@ procedure {:yields} {:layer 1} {:refines "AtomicRemoteIncrementBody"} RemoteIncr
     }
     yield;
 }
-procedure {:atomic} {:layer 2} AtomicRemoteIncrementBody(i: int)
+procedure {:atomic} {:layer 2} AtomicRemoteIncrementBody(i: int, phase: int)
 modifies done, x, Addrs;
 {
-    assert done[i] || Addrs[i];
-    if (!done[i]) {
-        done[i] := true;
+    assert done[i] >= phase || Addrs[i];
+    if (done[i] < phase) {
+        done[i] := phase;
 	x[i] := x[i] + 1;
 	Addrs[i] := false;
     }
 }
 
-procedure {:yields} {:layer 1} {:refines "AtomicRemoteMultiplyBody"} RemoteMultiplyBody(i: int)
+procedure {:yields} {:layer 1} {:refines "AtomicRemoteMultiplyBody"} RemoteMultiplyBody(i: int, phase: int)
 {
     var {:linear "addr1"} j: int;
     var {:linear "addr1"} x: Addr;
     yield;
-    call x := DoneUpdate(i);
+    call x := DoneUpdate(i, phase);
     if (is#Some(x)) {
         call j := Extract(x);   
         call Multiply(j);
     }
     yield;
 }
-procedure {:atomic} {:layer 2} AtomicRemoteMultiplyBody(i: int)
+procedure {:atomic} {:layer 2} AtomicRemoteMultiplyBody(i: int, phase: int)
 modifies done, x, Addrs;
 {
-    assert done[i] || Addrs[i];
-    if (!done[i]) {
-        done[i] := true;
+    assert done[i] >= phase || Addrs[i];
+    if (done[i] < phase) {
+        done[i] := phase;
 	x[i] := 2*x[i];
 	Addrs[i] := false;
     }
@@ -126,87 +126,87 @@ type Op;
 const unique INCREMENT: Op;
 const unique MULTIPLY: Op;
 
-procedure {:yields} {:layer 2} DuplicateRemote(i: int, op: Op)
-requires {:layer 2} done[i];
+procedure {:yields} {:layer 2} DuplicateRemote(i: int, op: Op, phase: int)
+requires {:layer 2} done[i] >= phase;
 {
     yield;
-    assert {:layer 2} done[i];
+    assert {:layer 2} done[i] >= phase;
     if (op == INCREMENT) {
-        call RemoteIncrementBody(i);
+        call RemoteIncrementBody(i, phase);
     } else if (op == MULTIPLY) {
-        call RemoteMultiplyBody(i);
+        call RemoteMultiplyBody(i, phase);
     }
     yield;
 }
 
-procedure {:yields} {:layer 2} {:refines "AtomicRemoteIncrement"} RemoteIncrement(i1: int, {:linear_in "addr2"} i2: int)
+procedure {:yields} {:layer 2} {:refines "AtomicRemoteIncrement"} RemoteIncrement(i1: int, {:linear_in "addr2"} i2: int, phase: int)
 {
     yield;
-    call RemoteIncrementBody(i1);
+    call RemoteIncrementBody(i1, phase);
     while (*)
     invariant {:terminates} {:layer 0,1,2} true;
     {
-        async call DuplicateRemote(i1, INCREMENT);
+        async call DuplicateRemote(i1, INCREMENT, phase);
     }
     yield;
 }
-procedure {:left} {:layer 3} AtomicRemoteIncrement(i1: int, {:linear_in "addr2"} i2: int)
+procedure {:left} {:layer 3} AtomicRemoteIncrement(i1: int, {:linear_in "addr2"} i2: int, phase: int)
 modifies done, x, Addrs;
 {
     assert i1 == i2;
-    assert !done[i1] && Addrs[i1];
-    done[i1] := true;
+    assert done[i1] < phase && Addrs[i1];
+    done[i1] := phase;
     x[i1] := x[i1] + 1;
     Addrs[i1] := false;
 }
 
-procedure {:yields} {:layer 2} {:refines "AtomicRemoteMultiply"} RemoteMultiply(i1: int, {:linear_in "addr2"} i2: int)
+procedure {:yields} {:layer 2} {:refines "AtomicRemoteMultiply"} RemoteMultiply(i1: int, {:linear_in "addr2"} i2: int, phase: int)
 {
     yield;
-    call RemoteMultiplyBody(i1);
+    call RemoteMultiplyBody(i1, phase);
     while (*)
     invariant {:terminates} {:layer 0,1,2} true;
     {
-        async call DuplicateRemote(i1, MULTIPLY);
+        async call DuplicateRemote(i1, MULTIPLY, phase);
     }
     yield;
 }
-procedure {:left} {:layer 3} AtomicRemoteMultiply(i1: int, {:linear_in "addr2"} i2: int)
+procedure {:left} {:layer 3} AtomicRemoteMultiply(i1: int, {:linear_in "addr2"} i2: int, phase: int)
 modifies done, x, Addrs;
 {
     assert i1 == i2;
-    assert !done[i1] && Addrs[i1];
-    done[i1] := true;
+    assert done[i1] < phase && Addrs[i1];
+    done[i1] := phase;
     x[i1] := 2*x[i1];
     Addrs[i1] := false;
 }
 
-procedure {:yields} {:layer 3} {:refines "AtomicLocalIncrement"} LocalIncrement({:linear_in "addr1"} i1: int, {:linear_in "addr2"} i2: int)
-requires {:layer 3} !done[i1];
+procedure {:yields} {:layer 3} {:refines "AtomicLocalIncrement"} LocalIncrement({:linear_in "addr1"} i1: int, {:linear_in "addr2"} i2: int, phase: int)
+requires {:layer 3} done[i1] < phase;
 {
     yield;
-    assert {:layer 3} !done[i1];    
-    call AddAddr(i1, i2);
-    async call RemoteIncrement(i1, i2);
+    assert {:layer 3} done[i1] < phase;
+    call AddAddr(i1, i2, phase);
+    async call RemoteIncrement(i1, i2, phase);
     yield;
 }
-procedure {:atomic} {:layer 4} AtomicLocalIncrement({:linear_in "addr1"} i1: int, {:linear_in "addr2"} i2: int)
+procedure {:atomic} {:layer 4} AtomicLocalIncrement({:linear_in "addr1"} i1: int, {:linear_in "addr2"} i2: int, phase: int)
 modifies x;
 {
     assert i1 == i2;
     x[i1] := x[i1] + 1;
 }
 
-procedure {:yields} {:layer 3} {:refines "AtomicLocalMultiply"} LocalMultiply({:linear_in "addr1"} i1: int, {:linear_in "addr2"} i2: int)
-requires {:layer 3} !done[i1];
+procedure {:yields} {:layer 3} {:refines "AtomicLocalMultiply"} LocalMultiply({:linear_in "addr1"} i1: int, {:linear_in "addr2"} i2: int, phase: int)
+requires {:layer 3} done[i1] < phase;
 {
     yield;
-    assert {:layer 3} !done[i1];    
-    call AddAddr(i1, i2);
-    async call RemoteMultiply(i1, i2);
+    assert {:layer 3} done[i1] < phase;
+    call AddAddr(i1, i2, phase);
+    async call RemoteMultiply(i1, i2, phase);
     yield;
 }
-procedure {:atomic} {:layer 4} AtomicLocalMultiply({:linear_in "addr1"} i1: int, {:linear_in "addr2"} i2: int)
+procedure {:atomic} {:layer 4} AtomicLocalMultiply({:linear_in "addr1"} i1: int, {:linear_in "addr2"} i2: int, phase: int)
 modifies x;
 {
     assert i1 == i2;
